StackToAssembly.thy
@@ -108,6 +108,9 @@ lemma [simp]: "(stack_to_mem (i2 # i3 # \<sigma>) \<mu>)(0 := 1 + int (length \<
       qed
   qed
 
+lemma [simp]: "\<Sigma>\<^sub>B \<in> state_convert \<Sigma>\<^sub>S \<Longrightarrow> b_assembly_output \<Sigma>\<^sub>B = stack_output \<Sigma>\<^sub>S"
+  by (induction \<Sigma>\<^sub>S rule: stack_output.induct, induction \<Sigma>\<^sub>B rule: b_assembly_output.induct) simp
+
 lemma eval_stack_conv [simp]: "eval_stack \<Pi> \<Sigma>\<^sub>S = Some \<Sigma>\<^sub>S' \<Longrightarrow> \<Sigma>\<^sub>A \<in> state_convert \<Sigma>\<^sub>S \<Longrightarrow> 
     \<exists>\<Sigma>\<^sub>A'. \<Sigma>\<^sub>A' \<in> state_convert \<Sigma>\<^sub>S' \<and> iterate (eval_b_assembly (program_convert \<Pi>)) \<Sigma>\<^sub>A \<Sigma>\<^sub>A'"
   proof (induction \<Pi> \<Sigma>\<^sub>S rule: eval_stack.induct)
@@ -333,18 +336,18 @@ lemma eval_stack_conv [simp]: "eval_stack \<Pi> \<Sigma>\<^sub>S = Some \<Sigma>
   qed
 
 theorem stack_to_assembly_correct [simp]: "iterate (eval_stack \<Pi>) \<Sigma>\<^sub>S \<Sigma>\<^sub>S' \<Longrightarrow> 
-  \<Sigma>\<^sub>A \<in> state_convert \<Sigma>\<^sub>S \<Longrightarrow> 
-    \<exists>\<Sigma>\<^sub>A'. \<Sigma>\<^sub>A' \<in> state_convert \<Sigma>\<^sub>S' \<and> iterate (eval_b_assembly (program_convert \<Pi>)) \<Sigma>\<^sub>A \<Sigma>\<^sub>A'"
-  proof (induction "eval_stack \<Pi>" \<Sigma>\<^sub>S \<Sigma>\<^sub>S' arbitrary: \<Sigma>\<^sub>A rule: iterate.induct)
+  \<Sigma>\<^sub>B \<in> state_convert \<Sigma>\<^sub>S \<Longrightarrow> 
+    \<exists>\<Sigma>\<^sub>B'. \<Sigma>\<^sub>B' \<in> state_convert \<Sigma>\<^sub>S' \<and> iterate (eval_b_assembly (program_convert \<Pi>)) \<Sigma>\<^sub>B \<Sigma>\<^sub>B'"
+  proof (induction "eval_stack \<Pi>" \<Sigma>\<^sub>S \<Sigma>\<^sub>S' arbitrary: \<Sigma>\<^sub>B rule: iterate.induct)
   case iter_refl
     thus ?case by fastforce
   next case (iter_step \<Sigma>\<^sub>S \<Sigma>\<^sub>S' \<Sigma>\<^sub>S'')
-    then obtain \<Sigma>\<^sub>A' where S: "\<Sigma>\<^sub>A' \<in> state_convert \<Sigma>\<^sub>S' \<and> 
-      iterate (eval_b_assembly (program_convert \<Pi>)) \<Sigma>\<^sub>A \<Sigma>\<^sub>A'" by blast
-    with iter_step eval_stack_conv obtain \<Sigma>\<^sub>A'' where
-        "\<Sigma>\<^sub>A'' \<in> state_convert \<Sigma>\<^sub>S'' \<and> iterate (eval_b_assembly (program_convert \<Pi>)) \<Sigma>\<^sub>A' \<Sigma>\<^sub>A''" 
+    then obtain \<Sigma>\<^sub>B' where S: "\<Sigma>\<^sub>B' \<in> state_convert \<Sigma>\<^sub>S' \<and> 
+      iterate (eval_b_assembly (program_convert \<Pi>)) \<Sigma>\<^sub>B \<Sigma>\<^sub>B'" by blast
+    with iter_step eval_stack_conv obtain \<Sigma>\<^sub>B'' where
+        "\<Sigma>\<^sub>B'' \<in> state_convert \<Sigma>\<^sub>S'' \<and> iterate (eval_b_assembly (program_convert \<Pi>)) \<Sigma>\<^sub>B' \<Sigma>\<^sub>B''" 
       by blast
-    with S have "\<Sigma>\<^sub>A'' \<in> state_convert \<Sigma>\<^sub>S'' \<and> iterate (eval_b_assembly (program_convert \<Pi>)) \<Sigma>\<^sub>A \<Sigma>\<^sub>A''" 
+    with S have "\<Sigma>\<^sub>B'' \<in> state_convert \<Sigma>\<^sub>S'' \<and> iterate (eval_b_assembly (program_convert \<Pi>)) \<Sigma>\<^sub>B \<Sigma>\<^sub>B''" 
       by fastforce
     thus ?case by blast
   qed
